proof/old_system/uni/algo_worklist/prop_completness.v
@@ -14,7 +14,7 @@ Hint Constructors a_wl_red : Hdb_a_wl_red_completness.
 
 
 Theorem d_a_wl_red_completness: forall Ω Γ,
-   Ω ⟶ᵈʷ⁎⋅ -> ⊢ᵃ Γ -> transfer Γ Ω  -> Γ ⟶ᵃʷ⁎⋅.
+   Ω ⟶ᵈʷ⁎⋅ -> ⊢ᵃʷ Γ -> transfer Γ Ω  -> Γ ⟶ᵃʷ⁎⋅.
 Proof with auto with Hdb_a_wl_red_completness.
   intros. generalize dependent Γ. induction H; auto. unfold transfer in *.
 Admitted.
